Foundation/ProvabilityLogic/Logic/Basic.lean
@@ -1,6 +1,6 @@
 module
 
-public import Foundation.ProvabilityLogic.Formula.Basic
+public import Foundation.ProvabilityLogic.Formula
 
 /-!
 # Logics
@@ -11,6 +11,72 @@ public import Foundation.ProvabilityLogic.Formula.Basic
 namespace FFL.ProvabilityLogic
 
 abbrev Logic (α : Type*) := Set (Formula α)
+
+open Formula
+
+variable {α : Type*}
+
+/-! ### Quasi-normal sums -/
+
+@[grind]
+inductive Logic.sumQuasiNormal (L₁ L₂ : Logic α) : Logic α
+  | mem₁ {A}    : A ∈ L₁ → sumQuasiNormal L₁ L₂ A
+  | mem₂ {A}    : A ∈ L₂ → sumQuasiNormal L₁ L₂ A
+  | mdp  {A B}  : sumQuasiNormal L₁ L₂ (A 🡒 B) → sumQuasiNormal L₁ L₂ A → sumQuasiNormal L₁ L₂ B
+  | subst {A s} : sumQuasiNormal L₁ L₂ A → sumQuasiNormal L₁ L₂ (A⟦s⟧)
+
+infix:50 " +ᴸ " => Logic.sumQuasiNormal
+
+namespace Logic.sumQuasiNormal
+
+variable {L₁ L₂ X Y : Logic α}
+
+@[grind .] lemma subset_left : L₁ ⊆ (L₁ +ᴸ L₂) := fun _ ↦ mem₁
+
+@[grind .] lemma subset_right : L₂ ⊆ (L₁ +ᴸ L₂) := fun _ ↦ mem₂
+
+lemma subset_iff : (L₁ +ᴸ X) ⊆ (L₁ +ᴸ Y) ↔ X ⊆ (L₁ +ᴸ Y) := by
+  constructor;
+  . intro h A hA;
+    exact h (mem₂ hA);
+  . intro h A hA;
+    induction hA with
+    | mem₁ hA => exact mem₁ hA;
+    | mem₂ hA => exact h hA;
+    | mdp _ _ ihAB ihA => exact mdp ihAB ihA;
+    | subst _ ih => exact subst ih;
+
+end Logic.sumQuasiNormal
+
+/-! ### Normal sums -/
+
+@[grind]
+inductive Logic.sumNormal (L₁ L₂ : Logic α) : Logic α
+  | mem₁ {A}    : A ∈ L₁ → sumNormal L₁ L₂ A
+  | mem₂ {A}    : A ∈ L₂ → sumNormal L₁ L₂ A
+  | mdp  {A B}  : sumNormal L₁ L₂ (A 🡒 B) → sumNormal L₁ L₂ A → sumNormal L₁ L₂ B
+  | subst {A s} : sumNormal L₁ L₂ A → sumNormal L₁ L₂ (A⟦s⟧)
+  | nec  {A}    : sumNormal L₁ L₂ A → sumNormal L₁ L₂ (□A)
+
+infix:50 " ⊕ᴸ " => Logic.sumNormal
+
+namespace Logic.sumNormal
+
+variable {L₁ L₂ : Logic α}
+
+@[grind .] lemma subset_left : L₁ ⊆ (L₁ ⊕ᴸ L₂) := fun _ ↦ mem₁
+
+@[grind .] lemma subset_right : L₂ ⊆ (L₁ ⊕ᴸ L₂) := fun _ ↦ mem₂
+
+lemma sumQuasiNormal_subset : (L₁ +ᴸ L₂) ⊆ (L₁ ⊕ᴸ L₂) := by
+  intro A h;
+  induction h with
+  | mem₁ h => exact mem₁ h;
+  | mem₂ h => exact mem₂ h;
+  | mdp _ _ ihAB ihA => exact mdp ihAB ihA;
+  | subst _ ih => exact subst ih;
+
+end Logic.sumNormal
 
 end FFL.ProvabilityLogic
 
