Foundation.lean
@@ -177,8 +177,7 @@ public import Foundation.Propositional.Logic.Basic
 public import Foundation.ProvabilityLogic.Arithmetic.GL.Basic
 public import Foundation.ProvabilityLogic.Arithmetic.Interpret
 public import Foundation.ProvabilityLogic.Arithmetic.SolovaySentences
-public import Foundation.ProvabilityLogic.Formula.Basic
-public import Foundation.ProvabilityLogic.Formula.Substitution
+public import Foundation.ProvabilityLogic.Formula
 public import Foundation.ProvabilityLogic.Gentzen.GL.Basic
 public import Foundation.ProvabilityLogic.Gentzen.GL.Kripke
 public import Foundation.ProvabilityLogic.Gentzen.Sequent
@@ -190,8 +189,6 @@ public import Foundation.ProvabilityLogic.Kripke.RootExtension
 public import Foundation.ProvabilityLogic.Kripke.RootedModel
 public import Foundation.ProvabilityLogic.Logic.Basic
 public import Foundation.ProvabilityLogic.Logic.GL.Basic
-public import Foundation.ProvabilityLogic.Logic.SumNormal
-public import Foundation.ProvabilityLogic.Logic.SumQuasiNormal
 public import Foundation.SecondOrder.LK.Basic
 public import Foundation.SecondOrder.Syntax.Formula
 public import Foundation.SecondOrder.Syntax.Rew
